src/tls/Model.CRF.fst
@@ -22,7 +22,13 @@ let h = Spec.Hash.hash
 open Mem 
 module MDM = FStar.Monotonic.DependentMap 
 
-type hashable (a:alg) = v:Seq.seq UInt8.t {Seq.length v < maxLength a}
+// now bounded irrespective of a, as in EverCrypt.Incremental (TBD)
+let bytes = Seq.seq UInt8.t
+
+//$ avoid using it because ghost lack structural subtyping.
+let hashable (s:bytes) = Seq.length s < pow2 61
+// type hashable (a:alg) = v:Seq.seq UInt8.t {Seq.length v < maxLength a}
+
 // the precise types guarantee that the table stays empty when crf _ = false
 private type range = | Computed: a: alg {crf a} -> t: tag a -> range
 private type domain (r:range) =
@@ -39,20 +45,34 @@ private let table : MDM.t tls_tables_region range domain inv = MDM.alloc()
 // (not sure how to manage that table)
 
 //val hashed: a:alg -> b:bytes -> Type
-abstract type hashed (a:alg) (b:hashable a) =
-  crf a ==> (
-    let t = h a b in
-    witnessed (MDM.contains table (Computed a t) (b <: domain (Computed a t))))
 
-val crf_injective (a:alg) (b0 b1:hashable a): ST unit  // should be STTot
-  (requires fun h0 -> hashed a b0 /\ hashed a b1)
-  (ensures fun h0 _ h1 -> h0 == h1 /\ (crf a /\ h a b0 == h a b1 ==> b0 == b1))
-let crf_injective a b0 b1 =
-  if crf a then (
+abstract type hashed (a:alg) (b:bytes) =
+  model /\ crf a ==> (
+    hashable b /\
+    Seq.length b < maxLength a /\
+    (
+    let t = h a b in
+    witnessed (MDM.contains table (Computed a t) (b <: domain (Computed a t)))))
+
+// required to go through abstraction when switching 
+let concrete_hashed a b: Lemma (~model ==> hashed a b) = ()
+
+val injective (a:alg) (b0 b1: Ghost.erased bytes): 
+  Stack unit  
+  (requires fun h0 -> 
+    let b0 = Ghost.reveal b0 in 
+    let b1 = Ghost.reveal b1 in
+    hashed a b0 /\ hashed a b1)
+  (ensures fun h0 _ h1 -> 
+    let b0 = Ghost.reveal b0 in 
+    let b1 = Ghost.reveal b1 in
+    h0 == h1 /\ (model /\ crf a /\ h a b0 == h a b1 ==> b0 == b1))
+let injective a b0 b1 =
+  if model && crf a then (
     recall table;
     let f = !table in
-    testify(MDM.contains table (Computed a (h a b0)) b0);
-    testify(MDM.contains table (Computed a (h a b1)) b1)
+    testify(MDM.contains table (Computed a (h a (Ghost.reveal b0))) (Ghost.reveal b0));
+    testify(MDM.contains table (Computed a (h a (Ghost.reveal b1))) (Ghost.reveal b1))
   )
 
 /// We use [stop] to model the exclusion of "bad" events, in this case
@@ -65,10 +85,11 @@ private val stop: s:string -> Stack 'a
   (ensures fun h0 r h1 -> False)
 let rec stop (s:string) = stop s
 
-val hash: a:alg -> v:hashable a -> Stack (tag a)
-  (requires fun h0 -> True)
+val hash: a:alg -> v:bytes -> Stack (tag a)
+  (requires fun h0 -> hashable v)
   (ensures fun h0 t h1 ->
     LowStar.Buffer.(modifies loc_none h0 h1) /\
+    Seq.length v < maxLength a /\
     t == h a v /\ 
     hashed a v
   )
@@ -79,6 +100,8 @@ module ST = FStar.HyperStack.ST
 
 let hash a v =
   let h0 = ST.get() in 
+  assert_norm (pow2 61 < pow2 125);
+  assert(Seq.length v < maxLength a);
   let t = Spec.Hash.hash a v in 
   if crf a then (
     let x = Computed a t in
@@ -94,10 +117,10 @@ let hash a v =
 // sanity check
 
 open FStar.Seq
-private val test (a:alg {crf a}) (b0 b1: hashable a): St unit
+private val test (a:alg {crf a}) (b0 b1: (b:bytes{hashable b})): St unit
 let test a b0 b1 =
   let t0 = hash a b0 in 
   let t1 = hash a b1 in
-  crf_injective a b0 b1;
-  if t0 = t1 then assert(b0 == b1)
+  injective a (Ghost.hide b0) (Ghost.hide b1);
+  if model && t0 = t1 then assert(b0 == b1)
   
